WasmInputs/dynamic_predule.wat
@@ -1,0 +1,86 @@
+(;;(module
+  (func $simple_add (result i32)
+    i32.const 5
+    i32.const 7
+    i32.add
+  )
+);)
+
+(;;(module
+  (func $cmp (param i32 i32) (result i32)
+    local.get 0
+    local.get 1
+    i32.lt_s
+  )
+);)
+(;;(module
+  (func $math (param f64) (result f64)
+    local.get 0
+    f64.sqrt
+    f64.floor
+    f64.abs
+  )
+);)
+
+(;;(module
+  (func $sel (param i32 i32 i32) (result i32)
+    local.get 0
+    local.get 1
+    local.get 2
+    select
+  )
+);)
+
+(module
+  (memory 1)
+  (func $load (result i32)
+    i32.const 0
+    i32.load
+  )
+)
+
+(;;(module
+  (memory 1)
+  (func $load8 (result i32)
+    i32.const 10
+    i32.load8_s
+  )
+);;)
+
+(;;(module
+  (func $loop_test (param i32) (result i32)
+    (local i32)
+    loop $L
+      local.get 0
+      i32.const 1
+      i32.sub
+      local.tee 0
+      br_if $L
+    end
+    local.get 0
+  )
+);;)
+
+(;;(module
+  (type $t0 (func (result i32)))
+  (table 1 funcref)
+
+  (func $f (result i32)
+    i32.const 0
+  )
+
+  (elem (i32.const 0) $f)
+
+  (func $indirect (result i32)
+    i32.const 0
+    call_indirect (type $t0)
+  )
+);)
+
+
+
+
+
+
+
+
